starting function definition

Weidenbach_Book/CDCL_Two_Watched_Literals_Implementation.thy
@@ -8,4 +8,119 @@ theory CDCL_Two_Watched_Literals_Implementation
 imports CDCL_Two_Watched_Literals
 begin
 
+locale state\<^sub>W_with_candidates =
+  state\<^sub>W trail init_clss learned_clss backtrack_lvl conflicting cons_trail tl_trail add_init_cls
+   add_learned_cls remove_cls update_backtrack_lvl update_conflicting init_state
+   restart_state
+  for     trail :: "'st \<Rightarrow> ('v, nat, 'v clause) marked_lits" and
+    init_clss :: "'st \<Rightarrow> 'v clauses" and
+    learned_clss :: "'st \<Rightarrow> 'v clauses" and
+    backtrack_lvl :: "'st \<Rightarrow> nat" and
+    conflicting :: "'st \<Rightarrow>'v clause conflicting_clause" and
+
+    cons_trail :: "('v, nat, 'v clause) marked_lit \<Rightarrow> 'st \<Rightarrow> 'st" and
+    tl_trail :: "'st \<Rightarrow>'st" and
+    add_init_cls :: "'v clause \<Rightarrow> 'st \<Rightarrow> 'st" and
+    add_learned_cls :: "'v clause \<Rightarrow> 'st \<Rightarrow> 'st" and
+    remove_cls :: "'v clause \<Rightarrow> 'st \<Rightarrow> 'st" and
+    update_backtrack_lvl :: "nat \<Rightarrow> 'st \<Rightarrow> 'st" and
+    update_conflicting :: "'v clause conflicting_clause \<Rightarrow> 'st \<Rightarrow> 'st" and
+
+    init_state :: "'v clauses \<Rightarrow> 'st" and
+    restart_state :: "'st \<Rightarrow> 'st" +
+  fixes
+    get_propagate_candidates :: "'st \<Rightarrow> ('v literal \<times> 'v clause) list" and
+    get_conflict_candidates :: "'st \<Rightarrow> 'v clause list" and
+    get_not_decided :: "'st \<Rightarrow> 'v literal option"
+  assumes
+    get_conflict_candidates_empty:
+      "\<And>S. get_conflict_candidates S = [] \<longleftrightarrow> (\<forall>D \<in># clauses S. \<not> trail S \<Turnstile>as CNot D)" and
+    get_conflict_candidates_in_clauses:
+      "\<And>S. \<forall>C \<in> set (get_conflict_candidates S). C \<in># clauses S \<and> trail S \<Turnstile>as CNot C" and
+    get_propagate_candidates_lit_in_cls:
+      "\<And>S. \<forall>(L, C) \<in> set (get_propagate_candidates S). undefined_lit (trail S) L \<and> C \<in># clauses S
+        \<and> trail S \<Turnstile>as CNot (C - {#L#}) \<and> L \<in># C" and
+    get_propagate_candidates_lit_empty:
+      "\<And>S. get_propagate_candidates S = [] \<longleftrightarrow>
+        \<not>(\<exists>C L. undefined_lit (trail S) L \<and> C + {#L#} \<in># clauses S \<and> trail S \<Turnstile>as CNot C)" and
+    get_not_decided_Some:
+      "\<And>S L. get_not_decided S = Some L \<Longrightarrow>
+         undefined_lit (trail S) L \<and> atm_of L \<in> atms_of_msu (init_clss S)" and
+    get_not_decided_None:
+      "\<And>S. get_not_decided S = None \<Longrightarrow>
+         \<not>(\<exists>L. undefined_lit (trail S) L \<and> atm_of L \<in> atms_of_msu (init_clss S))"
+
+locale
+  cdcl\<^sub>W_cands =
+   state\<^sub>W_with_candidates trail init_clss learned_clss backtrack_lvl conflicting cons_trail tl_trail
+   add_init_cls add_learned_cls remove_cls update_backtrack_lvl update_conflicting init_state
+   restart_state get_propagate_candidates get_conflict_candidates
+  for
+    trail :: "'st \<Rightarrow> ('v::linorder, nat, 'v::linorder clause) marked_lits" and
+    init_clss :: "'st \<Rightarrow> 'v clauses" and
+    learned_clss :: "'st \<Rightarrow> 'v clauses" and
+    backtrack_lvl :: "'st \<Rightarrow> nat" and
+    conflicting :: "'st \<Rightarrow>'v clause conflicting_clause" and
+
+    cons_trail :: "('v, nat, 'v clause) marked_lit \<Rightarrow> 'st \<Rightarrow> 'st" and
+    tl_trail :: "'st \<Rightarrow> 'st" and
+    add_init_cls :: "'v clause \<Rightarrow> 'st \<Rightarrow> 'st" and
+    add_learned_cls :: "'v clause \<Rightarrow> 'st \<Rightarrow> 'st" and
+    remove_cls :: "'v clause \<Rightarrow> 'st \<Rightarrow> 'st" and
+    update_backtrack_lvl :: "nat \<Rightarrow> 'st \<Rightarrow> 'st" and
+    update_conflicting :: "'v clause conflicting_clause \<Rightarrow> 'st \<Rightarrow> 'st" and
+
+    init_state :: "'v clauses \<Rightarrow> 'st" and
+    restart_state :: "'st \<Rightarrow> 'st" and
+    get_propagate_candidates :: "'st \<Rightarrow> ('v literal \<times> 'v clause) list" and
+    get_conflict_candidates :: "'st \<Rightarrow> 'v clause list"
+begin
+sublocale cdcl\<^sub>W_termination trail init_clss learned_clss backtrack_lvl conflicting cons_trail
+  tl_trail add_init_cls add_learned_cls remove_cls update_backtrack_lvl update_conflicting
+  init_state restart_state
+ by unfold_locales
+
+definition do_conflict_step :: "'st \<Rightarrow> 'st option" where
+"do_conflict_step S =
+  (case conflicting S of
+    C_Clause _ \<Rightarrow> None
+  | C_True \<Rightarrow>
+      (case get_conflict_candidates S of
+        [] \<Rightarrow> None
+      | a # _ \<Rightarrow> Some (update_conflicting (C_Clause a) S)))"
+
+lemma do_conflict_step_Some:
+  assumes conf: "do_conflict_step S = Some T"
+  shows "conflict S T"
+proof (cases "conflicting S")
+  case C_Clause
+  then show ?thesis using conf unfolding do_conflict_step_def by simp
+next
+  case C_True
+  then obtain C where
+    C: "C \<in> set (get_conflict_candidates S)" and
+    T: "T = update_conflicting (C_Clause C) S"
+     using conf unfolding do_conflict_step_def by (auto split: list.splits)
+  have "C \<in># clauses S" and "trail S \<Turnstile>as CNot C"
+    using get_conflict_candidates_in_clauses by (simp_all add: C some_in_eq)
+  then show ?thesis
+    using conflict_rule[of S _ _ _ _ C T]  state_eq_ref T C_True
+    by auto
+qed
+
+lemma do_conflict_step_None:
+  assumes conf: "do_conflict_step S = None"
+  shows "no_step conflict S"
+proof (cases "conflicting S")
+  case C_Clause
+  then show ?thesis by auto
+next
+  case C_True
+  then have "get_conflict_candidates S = []"
+     using conf unfolding do_conflict_step_def by (auto split: list.splits)
+  then show ?thesis
+    using get_conflict_candidates_empty by auto
+qed
+
+end
 end
